bind_base completed somewhat

our_cook/encoding.v
@@ -18,6 +18,9 @@ Fixpoint findRef (n : nat) (refs : list (nat * nat)) :=
       then y
       else findRef n ps
   end.
+  
+Definition pointer (p : proc) :=
+  Rep (In 0 (In 0 (In 1 p))).
 
 Fixpoint encode (s : term) (u r : nat) (refs : list (nat * nat)) :=
   match s with
@@ -32,29 +35,35 @@ Fixpoint encode (s : term) (u r : nat) (refs : list (nat * nat)) :=
       ))))))
       (Par
         (encode s 3 2 (incRefs 0 4 refs))
-        (encode_value v 1 0 (incRefs 0 4 refs))
+        (Out 1 (encode_value v (incRefs 0 4 refs)))
       )
     )
   | Force v => (Res ^^ 2) (Par
-      (encode_value v 1 0 (incRefs 0 2 refs))
+      (Out 1 (encode_value v (incRefs 0 2 refs)))
       (In 1 (Out 0 (Out 0 (Out 1 (Par
         (Link 1 (u + 6))
         (Link 0 (r + 6))
       )))))
     )
-  | Ret v => encode_value v r r refs
+  | Ret v => Out r (encode_value v refs)
   | Bind s t => (Res ^^ 2) (Par
       (encode s 1 0 (incRefs 0 2 refs))
       (In 0 (encode t (u + 3) (r + 3) (incRefs 1 3 refs)))
     )
-  | Val v => encode_value v u r refs
+  | Val v => Out u (encode_value v refs)
   end
 
-with encode_value (v : value) (u r : nat) (refs : list (nat * nat)) :=
-  match v with
-  | Var n => Out u (Rep (In 0 (In 0 (In 1 (In (n + 4) (In 0 (In 1 (Par
-      (Link 1 4)
-      (Link 0 3)
-    ))))))))
-  | Thunk s => Out u (Rep (In 0 (In 0 (In 1 (encode s 1 0 (incRefs 0 4 refs))))))
-  end.
+with encode_value (v : value) (refs : list (nat * nat)) :=
+  pointer(
+    match v with
+    | Var n => In (n + 4) (In 0 (In 1 (Par
+        (Link 1 4)
+        (Link 0 3)
+      )))
+    | Thunk s => encode s 1 0 (incRefs 0 4 refs)
+    end
+  ).
+  
+Notation "$ v ; refs $" := (encode_value v refs) (at level 90, left associativity).
+
+Notation "$ s ; u ; r ; refs $" := (encode s u r refs) (at level 90, left associativity).
